hop

src/lowparse/steel_st_array/LowParse.SteelST.Access.fst
@@ -25,6 +25,72 @@ let jumper
         SZ.size_v res == consumed
 )
 
+let hop_arrayptr_aparse
+  (#k: parser_kind)
+  (#t: Type)
+  (p: parser k t)
+  (#va1: _)
+  (#va2: _)
+  (a1: byte_array)
+  (sz: SZ.size_t)
+  (a2: Ghost.erased byte_array)
+: ST byte_array
+    (AP.arrayptr a1 va1 `star` aparse p a2 va2)
+    (fun res -> AP.arrayptr a1 va1 `star` aparse p res va2)
+    (AP.adjacent (AP.array_of va1) (array_of va2) /\ SZ.size_v sz == AP.length (AP.array_of va1))
+    (fun res -> res == Ghost.reveal a2)
+= let _ = elim_aparse p a2 in
+  let res = AP.split' a1 sz a2 in
+  let _ = gen_elim () in
+  let va2' = intro_aparse p res in
+  rewrite (aparse p res va2') (aparse p res va2);
+  return res
+
+let hop_aparse_arrayptr
+  (#k: parser_kind)
+  (#t: Type)
+  (#p: parser k t)
+  (j: jumper p)
+  (#va1: _)
+  (#va2: _)
+  (a1: byte_array)
+  (a2: Ghost.erased byte_array)
+: ST byte_array
+    (aparse p a1 va1 `star` AP.arrayptr a2 va2)
+    (fun res -> aparse p a1 va1 `star` AP.arrayptr res va2)
+    (AP.adjacent (array_of va1) (AP.array_of va2))
+    (fun res -> res == Ghost.reveal a2)
+= let _ = elim_aparse p a1 in
+  let sz = j a1 in
+  let res = AP.split' a1 sz a2 in
+  let _ = gen_elim () in
+  let va1' = intro_aparse p a1 in
+  rewrite (aparse p a1 va1') (aparse p a1 va1);
+  return res
+
+let hop_aparse_aparse
+  (#k1: parser_kind)
+  (#t1: Type)
+  (#p1: parser k1 t1)
+  (j1: jumper p1)
+  (#k2: _)
+  (#t2: _)
+  (p2: parser k2 t2)
+  (#va1: _)
+  (#va2: _)
+  (a1: byte_array)
+  (a2: Ghost.erased byte_array)
+: ST byte_array
+    (aparse p1 a1 va1 `star` aparse p2 a2 va2)
+    (fun res -> aparse p1 a1 va1 `star` aparse p2 res va2)
+    (AP.adjacent (array_of va1) (array_of va2))
+    (fun res -> res == Ghost.reveal a2)
+= let _ = elim_aparse p2 a2 in
+  let res = hop_aparse_arrayptr j1 a1 a2 in
+  let va2' = intro_aparse p2 res in
+  rewrite (aparse p2 res va2') (aparse p2 res va2);
+  return res
+
 let jump_constant_size
   (#k: parser_kind)
   (#t: Type)
